theories/opsem.v
@@ -26,6 +26,21 @@ Fixpoint isla_trace_length (t : isla_trace) : nat :=
   | tfork ts => S (sum_list (isla_trace_length <$> ts))
   end.
 
+Definition false_trace : isla_trace := Assume (AExp_Val (AVal_Bool false) Mk_annot) Mk_annot:t:tnil.
+
+Definition partial_trace (v : base_val) (t : isla_trace) : isla_trace :=
+  match t with
+  | Smt (DeclareConst x (Ty_BitVec n)) _ :t: t' =>
+      match v with
+      | Val_Bits b =>
+          if (b.(bvn_n) =? n)%N then subst_trace v x t' else false_trace
+      | _ => false_trace
+      end
+  | Smt (DeclareConst x Ty_Bool) _ :t: t' =>
+      if v is Val_Bool _ then subst_trace v x t' else false_trace
+  | _ => false_trace
+  end.
+
 Global Instance valu_inhabited : Inhabited valu := populate (RVal_Bool true).
 Global Instance enum_id_eq_decision : EqDecision enum_id.
 Proof. solve_decision. Qed.
