examples/partial.v
@@ -1,0 +1,22 @@
+Require Import isla.aarch64.aarch64.
+From isla.instructions.partial Require Import instrs.
+
+Section proof.
+Context `{!islaG Σ} `{!threadG}.
+
+Lemma partial_spec :
+  instr 0x0000000010300000 (Some (partial_trace (Val_Bits (bv_0 16)) (partial_trace (Val_Bits (bv_0 2)) a7428))) -∗
+  instr_body 0x0000000010300000 (
+    ∃ (b : bv 64),
+    "R0" ↦ᵣ RVal_Bits b ∗
+    instr_pre 0x0000000010300004 (
+      "R0" ↦ᵣ RVal_Bits b ∗
+      True
+  )).
+Proof.
+  iStartProof.
+  repeat liAStep; liShow.
+  Unshelve. all: prepare_sidecond.
+  (* all: try bv_solve. *)
+  - bv_simplify.
+Abort.
