instructions/partial/instrs.v
@@ -1,0 +1,6 @@
+Require Import isla.isla_lang.
+Require Export isla.instructions.partial.a7428.
+
+Definition instr_map := [
+  (0x7428%Z, a7428 (* mov x6, #0x0 *))
+].
